analysis/Analysis/Section_3_1.lean
@@ -90,6 +90,7 @@ instance SetTheory.Set.instEmpty : EmptyCollection Set where
   emptyCollection := SetTheory.emptyset
 
 /-- Axiom 3.3 (empty set).  Note: one may have to explicitly cast ∅ to Set due to Mathlib's existing set theory notation. -/
+@[simp]
 theorem SetTheory.Set.not_mem_empty : ∀ x, x ∉ (∅:Set) := SetTheory.emptyset_mem
 
 /-- Empty set is unique -/
@@ -113,6 +114,7 @@ instance SetTheory.Set.instSingleton : Singleton Object Set where
   singleton := SetTheory.singleton
 
 /-- Axiom 3.3(a) (singleton).  Note one may have to explicitly cast {a} to Set due to Mathlib's existing set theory notation. -/
+@[simp]
 theorem SetTheory.Set.mem_singleton (x a:Object) : x ∈ ({a}:Set) ↔ x = a := by
   exact SetTheory.singleton_axiom x a
 
@@ -130,6 +132,7 @@ instance SetTheory.Set.instInsert : Insert Object Set where
 theorem SetTheory.Set.pair_eq (a b:Object) : ({a,b}:Set) = {a} ∪ {b} := by rfl
 
 /-- Axiom 3.3(b) (pair).  Note that one often has to cast {a,b} to Set -/
+@[simp]
 theorem SetTheory.Set.mem_pair (x a b:Object) : x ∈ ({a,b}:Set) ↔ (x = a ∨ x = b) := by
   rw [pair_eq, mem_union, mem_singleton, mem_singleton]
 
@@ -295,6 +298,7 @@ instance SetTheory.Set.instIntersection : Inter Set where
   inter X Y := X.specify (fun x ↦ x.val ∈ Y)
 
 /-- Definition 3.1.22 (Intersections) -/
+@[simp]
 theorem SetTheory.Set.mem_inter (x:Object) (X Y:Set) : x ∈ (X ∩ Y) ↔ (x ∈ X ∧ x ∈ Y) := by
   constructor
   . intro h
@@ -308,6 +312,7 @@ instance SetTheory.Set.instSDiff : SDiff Set where
   sdiff X Y := X.specify (fun x ↦ x.val ∉ Y)
 
 /-- Definition 3.1.26 (Difference sets) -/
+@[simp]
 theorem SetTheory.Set.mem_sdiff (x:Object) (X Y:Set) : x ∈ (X \ Y) ↔ (x ∈ X ∧ x ∉ Y) := by
   constructor
   . intro h
@@ -430,6 +435,11 @@ theorem SetTheory.Set.ofNat_inj' (n m:ℕ) :
     (ofNat(n) : Object) = (ofNat(m) : Object) ↔ ofNat(n) = ofNat(m) := by
       simp only [←Object.ofnat_eq, Object.ofnat_eq', Set.coe_inj, Set.nat_equiv_inj]
       rfl
+
+@[simp]
+theorem SetTheory.Object.natCast_inj (n m:ℕ) :
+    (n : Object) = (m : Object) ↔ n = m := by
+      simp [←ofnat_eq, Subtype.val_inj]
 
 @[simp]
 lemma SetTheory.Set.nat_equiv_coe_of_coe (n:ℕ) : ((n:Nat):ℕ) = n := Equiv.symm_apply_apply nat_equiv n
